compiler/dafny_new/semantics/dafny_freshenProofScript.sml
@@ -8,7 +8,7 @@ open mlstringTheory
 open mlintTheory
 open dafny_evaluateTheory
 open dafny_semanticPrimitivesTheory
-open quantHeuristicsTheory  (* LIST_LENGTH_1 *)
+open dafny_evaluatePropsTheory
 
 val _ = new_theory "dafny_freshenProof";
 
@@ -521,124 +521,6 @@ Proof
   \\ gvs [add_fresh_def]
 QED
 
-(* Lemmas about length of locals. *)
-
-Triviality freshen_exps_len_eq:
-  ∀m cnt es cnt' es'.
-    freshen_exps m cnt es = (cnt', es') ⇒ LENGTH es = LENGTH es'
-Proof
-  Induct_on ‘es’ \\ rpt strip_tac
-  \\ gvs [freshen_exp_def] \\ rpt (pairarg_tac \\ gvs[]) \\ res_tac
-QED
-
-Triviality declare_local_len_inc:
-  ∀s v. LENGTH (declare_local s v).locals = LENGTH s.locals + 1
-Proof
-  gvs [declare_local_def]
-QED
-
-Triviality pop_local_len_dec:
-  ∀s s'. pop_local s = SOME s' ⇒ LENGTH s'.locals = LENGTH s.locals - 1
-Proof
-  rpt strip_tac \\ gvs [pop_local_def, AllCaseEqs()]
-QED
-
-Triviality locals_not_empty_pop_locals_some:
-  ∀s. 0 < LENGTH s.locals ⇒ ∃s'. pop_local s = SOME s'
-Proof
-  rpt strip_tac \\ gvs [pop_local_def, LIST_LENGTH_1]
-QED
-
-Triviality evaluate_exp_len_locals:
-  (∀s env e s' r.
-     evaluate_exp s env e = (s', r) ⇒ LENGTH s'.locals = LENGTH s.locals) ∧
-  (∀s env es s' r.
-     evaluate_exps s env es = (s', r) ⇒ LENGTH s'.locals = LENGTH s.locals)
-Proof
-  ho_match_mp_tac evaluate_exp_ind \\ rpt strip_tac
-  \\ gvs [evaluate_exp_def, set_up_call_def, restore_locals_def, AllCaseEqs()]
-QED
-
-Triviality update_local_aux_len_locals:
-  ∀locals var val locals'.
-    update_local_aux locals var val = SOME locals' ⇒
-    LENGTH locals = LENGTH locals'
-Proof
-  Induct_on ‘locals’ \\ rpt strip_tac
-  \\ gvs [update_local_aux_def] \\ PairCases_on ‘h’
-  \\ gvs [update_local_aux_def, AllCaseEqs()] \\ res_tac
-QED
-
-Triviality update_local_len_locals:
-  ∀s var val s'.
-    update_local s var val = SOME s' ⇒
-    LENGTH s'.locals = LENGTH s.locals
-Proof
-  rpt strip_tac
-  \\ gvs [update_local_def, AllCaseEqs()]
-  \\ imp_res_tac update_local_aux_len_locals \\ gvs []
-QED
-
-Triviality assign_value_len_locals:
-  ∀s env lhs rhs s' r.
-    assign_value s env lhs rhs = (s', r) ⇒
-    LENGTH s'.locals = LENGTH s.locals
-Proof
-  Cases_on ‘lhs’ \\ rpt strip_tac
-  \\ gvs [assign_value_def, update_array_def, AllCaseEqs()]
-  \\ imp_res_tac evaluate_exp_len_locals \\ gvs []
-  \\ imp_res_tac update_local_len_locals
-QED
-
-Triviality assign_values_len_locals:
-  ∀s env lhss vals s' r.
-    assign_values s env lhss vals = (s', r) ⇒
-    LENGTH s'.locals = LENGTH s.locals
-Proof
-  Induct_on ‘lhss’ \\ Cases_on ‘vals’ \\ rpt strip_tac
-  \\ gvs [assign_values_def, AllCaseEqs()]
-  \\ imp_res_tac assign_value_len_locals \\ res_tac \\ gvs []
-QED
-
-Triviality evaluate_rhs_exp_len_locals:
-  ∀s env e.
-    evaluate_rhs_exp s env e = (s', r) ⇒
-    LENGTH s'.locals = LENGTH s.locals
-Proof
-  Cases_on ‘e’ \\ rpt strip_tac
-  \\ gvs [evaluate_rhs_exp_def, alloc_array_def, AllCaseEqs()]
-  \\ imp_res_tac evaluate_exp_len_locals \\ gvs []
-QED
-
-Triviality evaluate_rhs_exps_len_locals:
-  ∀s env es s' r.
-    evaluate_rhs_exps s env es = (s', r) ⇒
-    LENGTH s'.locals = LENGTH s.locals
-Proof
-  Induct_on ‘es’ \\ rpt strip_tac
-  \\ gvs [evaluate_rhs_exps_def, AllCaseEqs ()]
-  \\ imp_res_tac evaluate_rhs_exp_len_locals \\ res_tac \\ gvs []
-QED
-
-Triviality evaluate_stmt_len_locals:
-  ∀s env scope s' r.
-    evaluate_stmt s env scope = (s', r) ⇒
-    LENGTH s'.locals = LENGTH s.locals
-Proof
-  ho_match_mp_tac evaluate_stmt_ind \\ rpt strip_tac
-  >~ [‘Dec local scope’] >-
-   (gvs [evaluate_stmt_def] \\ rpt (pairarg_tac \\ gvs [])
-    \\ gvs [declare_local_len_inc, AllCaseEqs()] \\ rename [‘pop_local s₁’]
-    >- (‘0 < LENGTH s₁.locals’ by gvs []
-        \\ imp_res_tac locals_not_empty_pop_locals_some \\ gvs [])
-    \\ imp_res_tac pop_local_len_dec \\ gvs [])
-  \\ gvs [evaluate_stmt_def, dec_clock_def, print_string_def,
-          restore_locals_def, set_up_call_def, AllCaseEqs()]
-  \\ imp_res_tac evaluate_exp_len_locals
-  \\ imp_res_tac assign_values_len_locals
-  \\ imp_res_tac evaluate_rhs_exps_len_locals \\ gvs []
-QED
-
 (* state_rel *)
 
 Triviality state_rel_mono:
@@ -689,6 +571,15 @@ Proof
   \\ namedCases_on ‘env'.prog’ ["members'"]
   \\ rpt strip_tac \\ gvs [get_member_def, freshen_program_def]
   \\ drule get_member_aux_some \\ gvs []
+QED
+
+(* freshen_exp *)
+Triviality freshen_exps_len_eq:
+  ∀m cnt es cnt' es'.
+    freshen_exps m cnt es = (cnt', es') ⇒ LENGTH es = LENGTH es'
+Proof
+  Induct_on ‘es’ \\ rpt strip_tac
+  \\ gvs [freshen_exp_def] \\ rpt (pairarg_tac \\ gvs[]) \\ res_tac
 QED
 
 (* Proving the main theorems, namely the correctness of the freshen pass. *)
@@ -1288,6 +1179,9 @@ Proof
    (gvs [evaluate_stmt_def, freshen_stmt_def]
     \\ rpt (pairarg_tac \\ gvs [])
     \\ gvs [evaluate_stmt_def]
+    \\ ‘env'.is_running = env.is_running’ by gvs [env_rel_def] \\ gvs []
+    \\ Cases_on ‘env.is_running’ \\ gvs []
+    >- (imp_res_tac freshen_exp_mono \\ imp_res_tac state_rel_mono)
     \\ namedCases_on ‘evaluate_exp s env e’ ["s₁ r"] \\ gvs []
     \\ namedCases_on ‘r’ ["v", "err"] \\ gvs []
     \\ drule (cj 1 correct_freshen_exp) \\ gvs [] \\ disch_then drule_all
