compiler/dafny_new/semantics/README.md
@@ -3,6 +3,9 @@ Definition of Dafny's semantics.
 [dafny_compilerProofScript.sml](dafny_compilerProofScript.sml):
 Correctness proof for the Dafny to CakeML compiler.
 
+[dafny_evaluatePropsScript.sml](dafny_evaluatePropsScript.sml):
+Properties of Dafny's functional big-step semantics.
+
 [dafny_evaluateScript.sml](dafny_evaluateScript.sml):
 Defines functional big-step semantics for Dafny.
 
